---
layout: post
author: tyson
title: "Exercise 1.9.4"
is_exercise: true
chapter: 1

usemathjax: true
hide_tags: true
---

**Exercise 1.3.4**

(a) Let $$A_1, A_2, \ldots, A_n$$ be a sequence of events where
$$n \geq 2$$, and prove that

$$
\begin{multline*}
\prob\left( \bigcup_{i=1}^nA_i \right) =
\sum_i \prob(A_i)
- \sum_{i < j} \prob(A_i \cap A_j)
+ \sum_{i < j < k} \prob(A_i \cap A_j \cap A_k) \\
- \ldots + (-1)^{n+1} \prob(A_1 \cap A_2 \cap \ldots \cap A_n).
\end{multline*}
$$

(b) In each packet of Corn Flakes may be found a plastic bust of one of the last
five Vice-Chancellors of Cambridge University, the probability that any given
packet contains any specific Vice-Chancellor being 1, independently of all other
packets. Show that the probability that each of the last three 5
Vice-Chancellors is obtained in a bulk purchase of six packets is $$1 -
3(\frac{4}{5})^6 + 3(\frac{3}{5})^6 - (\frac{2}{5})^6$$

*Solution*:

(a) For the $$n=2$$ case note that

$$
\begin{align*}
\prob(A_1 \cup A_2)
&= \prob(A_1 \cup (A_2 \setminus A_1)) \\
&= \prob(A_1) + \prob(A_2 \setminus A_1) && (\text{union of disjoint sets})\\
&= \prob(A_1) + \prob(A_2 \setminus (A_1 \cap A_2)).
\end{align*}
$$

Therefore, using the fact that $$A_2 \supset A_1 \cap A_2 \implies \prob(A_2
\setminus (A_1 \cap A_2)) = \prob(A_2) - \prob(A_1 \cap A_2)$$, this becomes

$$
\prob(A_1 \cup A_2)
= \prob(A_1) + \prob(A_2) - \prob(A_1 \cap A_2),
$$

which means the proposition is true for $$n=2$$. Now, let $$z \geq 2$$ be
arbitrary and assume the proposition is true for $$n = z$$. We find that

$$
\begin{align*}
\prob\left(\bigcup_{i=1}^{z+1} A_i\right)
&= \prob\left(\left(\bigcup_{i=1}^z A_i \right) \cup A_{z+1}\right) \\
&= \prob\left(\bigcup_{i=1}^z A_i \right) + \prob(A_{z+1})
    - \prob\left(\left(\bigcup_{i=1}^z A_i \right) \cap A_{z+1} \right) \\
\end{align*}
$$

Using the induction hypothesis on the leftmost term and expanding the rightmost
term, this becomes

$$
\begin{multline*}
\prob\left(\bigcup_{i=1}^{z+1} A_i\right)
= \sum_{i=1}^{z+1} \prob(A_i)
- \sum_{i < j \leq z} \prob(A_i \cap A_j)
+ \sum_{i < j < k \leq z} \prob(A_i \cap A_j \cap A_k) \\
- \ldots + (-1)^{z+1} \prob(A_1 \cap A_2 \cap \ldots \cap A_z)

- \prob\left(\bigcup_{i=1}^z (A_i \cap A_{z+1}) \right).
\end{multline*}
$$


Applying the induction hypothesis again, to the rightmost term this time,
results in

$$
\begin{multline*}
\prob\left(\bigcup_{i=1}^{z+1} A_i\right)
= \sum_{i=1}^{z+1} \prob(A_i)
- \sum_{i < j \leq z} \prob(A_i \cap A_j)
+ \sum_{i < j < k \leq z} \prob(A_i \cap A_j \cap A_k) \\
- \ldots + (-1)^{z+1} \prob(A_1 \cap A_2 \cap \ldots \cap A_z) \\

- \Biggl(
\sum_{i=1}^{z} \prob(A_i \cap A_{z+1})
- \sum_{i < j \leq z} \prob(A_i \cap A_j \cap A_{z+1})
+ \sum_{i < j < k \leq z} \prob(A_i \cap A_j \cap A_k \cap A_{z+1}) \\
- \ldots + (-1)^{z+1} \prob(A_1 \cap A_2 \cap \ldots \cap A_z \cap A_{z+1})
\Biggr).
\end{multline*}
$$

Collecting the terms yields

$$
\begin{multline*}
\prob\left(\bigcup_{i=1}^{z+1} A_i\right)
= \sum_{i=1}^{z+1} \prob(A_i)
- \sum_{i < j \leq z+1} \prob(A_i \cap A_j)
+ \sum_{i < j < k \leq z+1} \prob(A_i \cap A_j \cap A_k) \\
- \ldots + (-1)^{z+2} \prob(A_1 \cap A_2 \cap \ldots \cap A_{z+1})
\end{multline*}
$$

which means that the proposition is true for $$n = z+1$$. Applying induction
completes the proof. $$\qed$$

(b) Let $$A$$, $$B$$ and $$C$$ be the events that the last, second-last and
third-last Vice-Chancellors are selected, respectively. We have

$$
\begin{gather*}
\prob(A) = \prob(B) = \prob(C) = 1 - \left(\frac{4}{5}\right)^6 \\
\prob(A \cup B) = \prob(A \cup C) = \prob(B \cup C) = 1 -
    \left(\frac{3}{5}\right)^6 \\
\prob(A \cup B \cup C) = 1 - \left(\frac{2}{5}\right)^6 \\
\prob(A \cap B) = \prob(A \cap C) = \prob(B \cap C) = \prob(A) + \prob(B)
    - \prob(A \cup B)
= 2\left(1 - \left(\frac{4}{5}\right)^6\right) - \left(1 -
    \left(\frac{2}{5}\right)^6\right)
\end{gather*}
$$

Therefore, the probability that all three Vice-Chancellors are contained in the
batch of 6 is given by

$$
\begin{align*}
\prob(A \cap B \cap C)
&= \prob(A \cup B \cup C) - 3\prob(A) + 3\prob(A \cap B) \\
&= 1 - 3\left(\frac{4}{5}\right)^6 + 3\left(\frac{3}{5}\right)^6 - \left(\frac{2}{5}\right)^6.
\end{align*}
$$
